Add the necessary well_formedness properties to L2/L3 and correct translation
- L2k strip params, so the entries for all inductives in the environment
  have their parameters turned to 0.
- In L3, for correct terms, the inductive annotation on cases matches an
  inductive declaration in the environment, and branches of the case
  have arities as declared in the environment.
  This correctness criterion is preserved by everything, as proven.

theories/L3_flattenedApp/program.v
@@ -51,14 +51,19 @@ Definition CrctBranches (e: environ Term) (brs: Defs) : Prop :=
     end.
  ***)
 
-Definition CrctAnnot
-    (e: environ Term) (ann: inductive * nat) (brs: Defs) : Prop :=
-  let '(ind, pars) := ann in
-  let 'mkInd mind n := ind in
-  match lookup mind e with
-  | Some (ecTyp _ pars' pack) => pars' = pars
-  | _ => False
-  end.
+Inductive match_annot : list Cnstr -> Brs -> Prop :=
+| match_annot_nil : match_annot nil bnil
+| match_annot_cons t args c cnstrs ds :
+    c.(CnstrArity) = args ->
+    match_annot cnstrs ds ->
+    match_annot (c :: cnstrs) (bcons args t ds).
+         
+Definition crctAnnot (e : environ Term) ann brs :=
+  let 'mkInd nm tndx := ann in
+  exists pack ityp,
+    LookupTyp nm e 0 pack /\
+    getInd pack tndx = Ret ityp /\
+    match_annot ityp.(itypCnstrs) brs.
 
 (** correctness specification for programs (including local closure) **)
 Inductive crctTerm: environ Term -> nat -> Term -> Prop :=
@@ -74,16 +79,17 @@ Inductive crctTerm: environ Term -> nat -> Term -> Prop :=
            crctTerm p n (TApp fn arg)
 | ctConst: forall p n pd nm,
              crctEnv p -> LookupDfn nm p pd -> crctTerm p n (TConst nm)
-| ctConstructor: forall p n ipkgNm inum cnum args ipkg itp cstr pars,
-                   LookupTyp ipkgNm p pars ipkg ->
+| ctConstructor: forall p n ipkgNm inum cnum args ipkg itp cstr,
+                   LookupTyp ipkgNm p 0 ipkg ->
                    getInd ipkg inum = Ret itp ->
                    getCnstr itp cnum = Ret cstr ->
                    CnstrArity cstr = tlength args ->
                    crctTerms p n args ->
                    crctTerm p n (TConstruct (mkInd ipkgNm inum) cnum args)
 | ctCase: forall p n i mch brs,
-            crctTerm p n mch -> crctBs p n brs ->
-            crctTerm p n (TCase i mch brs)
+    crctTerm p n mch -> crctBs p n brs ->
+    crctAnnot p i brs ->
+    crctTerm p n (TCase i mch brs)
 | ctFix: forall p n ds m,
            crctDs p (n + dlength ds) ds -> m < dlength ds ->
            crctTerm p n (TFix ds m)
@@ -206,10 +212,14 @@ Proof.
   - unfold LookupDfn in H1. elim (Lookup_fresh_neq H1 H2). reflexivity.
   - unfold LookupTyp in H. destruct H.
     elim (Lookup_fresh_neq H H5). reflexivity.
+  - specialize (H2 _ H4). contradiction.
+  - destruct H3 as (pack&ityp&Hlook&_).
+    unfold LookupTyp in Hlook. destruct Hlook.
+    elim (Lookup_fresh_neq H3 H4). reflexivity.
   - specialize (H0 _ H2). contradiction.
   - specialize (H2 _ H4). contradiction.
   - inversion H6. 
-Qed.    
+Qed.
 
 Lemma Crct_weaken:
   (forall p n t, crctTerm p n t -> 
@@ -233,6 +243,10 @@ Proof.
     apply neq_sym. apply (Lookup_fresh_neq H1 H2). eassumption.
   - destruct H. unfold LookupTyp. split; try eassumption.
     constructor; try eassumption.
+    apply neq_sym. eapply Lookup_fresh_neq; eassumption.
+  - red. red in H3. destruct i. destruct H3 as [pack [ityp0 [Hlook [Hget Hann]]]].
+    exists pack. exists ityp0. intuition.
+    destruct Hlook. split; auto. constructor; auto.
     apply neq_sym. eapply Lookup_fresh_neq; eassumption.
 Qed.
 
@@ -258,7 +272,11 @@ Proof.
     apply neq_sym. apply (Lookup_fresh_neq H1 H2). eassumption.
   - unfold LookupTyp in *. destruct H. split; try eassumption.
     constructor; try eassumption.
-    apply neq_sym. apply (Lookup_fresh_neq l). assumption.
+    apply neq_sym. apply (Lookup_fresh_neq H). assumption.
+  - red. red in H3. destruct i. destruct H3 as [pack [ityp0 [Hlook [Hget Hann]]]].
+    exists pack. exists ityp0. intuition.
+    destruct Hlook. split; auto. constructor; auto.
+    apply neq_sym. eapply Lookup_fresh_neq; eassumption.
 Qed.
 
 Lemma Crct_strengthen:
@@ -297,9 +315,13 @@ Proof.
     + eapply H4. reflexivity. intros h. elim H6. apply PoCnstrA.
       assumption.
   - econstructor; try eassumption.
-    + eapply H0. reflexivity. intros h. elim H4. constructor. assumption.
-    + eapply H2. reflexivity. intros h. elim H4.
+    + eapply H0. reflexivity. intros h. elim H5. constructor. assumption.
+    + eapply H2. reflexivity. intros h. elim H5.
       apply PoCaseR. assumption.
+    + destruct i. destruct H3 as (pack&ityp&Hlook&Hget&Hann).
+      exists pack, ityp. split; auto.
+      destruct Hlook as [Hlook Hnil]. split; auto.
+      inversion Hlook; subst. elim H5. apply PoCaseAnn. assumption.
   - econstructor; try eassumption. eapply H0. reflexivity. intros h.
     elim H3. constructor. assumption.
   - constructor.
@@ -423,7 +445,7 @@ Qed.
 
 Lemma Crct_invrt_Case:
   forall p n i s us,
-    crctTerm p n (TCase i s us) -> crctTerm p n s /\ crctBs p n us.
+    crctTerm p n (TCase i s us) -> crctTerm p n s /\ crctBs p n us /\ crctAnnot p i us.
 Proof.
    intros. inversion_Clear H. intuition.
 Qed.
@@ -439,12 +461,13 @@ Lemma Crct_invrt_Construct:
   forall p n ipkgNm inum cnum args,
     crctTerm p n (TConstruct (mkInd ipkgNm inum) cnum args) ->
     crctTerms p n args /\
-    exists npars itypk,
-      LookupTyp ipkgNm p npars itypk /\
+    exists itypk,
+      LookupTyp ipkgNm p 0 itypk /\
       exists (ip:ityp), getInd itypk inum = Ret ip /\
-                   exists (ctr:Cnstr), getCnstr ip cnum = Ret ctr.
+                        exists (ctr:Cnstr), getCnstr ip cnum = Ret ctr /\
+                                            CnstrArity ctr = tlength args.
 Proof.
-  intros. inversion_Clear H. intuition. exists pars, ipkg. intuition.
+  intros. inversion_Clear H. intuition. exists ipkg. intuition.
   exists itp. intuition. exists cstr. intuition.
 Qed.
 
@@ -542,6 +565,11 @@ Proof.
   - inversion_Clear H2. constructor; try assumption.
     + apply H; try eassumption.
     + apply H0; try eassumption.
+    + destruct i as [ind k].
+      destruct H11 as (pack&ityp&Hlook&Hget&Hann).
+      exists pack, ityp; intuition auto.
+      destruct ityp. simpl in *. clear H H0; revert Hann its i1; clear.
+      induction 1; inversion_clear 1; constructor; auto.
   - pose proof (InstantiateDefs_pres_dlength i) as k.
     inversion_Clear H1. constructor; try omega. apply H. omega.
     + replace (S (m0 + dlength id)) with (S m0 + dlength d); try omega.
